pulse/lib/steel/pulse/Pulse.Checker.Pure.fsti
@@ -14,12 +14,6 @@ module RU = Pulse.RuntimeUtils
 let push_context (ctx:string) (r:range) (g:env) : (g':env { g == g' })
   = push_context g ctx r
 
-val print_context (g:env) : T.Tac string
-
-val print_issue (g:env) (i:FStar.Issue.issue) : T.Tac string
-
-val print_issues (g:env) (i:list FStar.Issue.issue) : T.Tac string
-
 val instantiate_term_implicits (g:env) (t:term)
   : T.Tac (term & term)
 
